

*Proof.* This is a direct application of the abstract Bayes formula. Assume first that  $\eta X$  is an  $\mathcal{F}$ -martingale under  $\mathbb{P}$  so that  $\mathbb{E}^{\mathbb{P}}(\eta_t X_t \mid \mathcal{F}_u) = \eta_u X_u$  for any  $0 \leq u \leq t \leq T$ . Then the Bayes formula yields,

$$\mathbb{E}^{\mathbb{Q}}(X_t \mid \mathcal{F}_u) = \frac{\mathbb{E}^{\mathbb{P}}(\eta_T X_t \mid \mathcal{F}_u)}{\mathbb{E}^{\mathbb{P}}(\eta_T \mid \mathcal{F}_u)} = \frac{\mathbb{E}^{\mathbb{P}}(X_t \mathbb{E}^{\mathbb{P}}(\eta_T \mid \mathcal{F}_t) \mid \mathcal{F}_u)}{\mathbb{E}^{\mathbb{P}}(\eta_T \mid \mathcal{F}_u)} = \frac{\mathbb{E}^{\mathbb{P}}(X_t \eta_t \mid \mathcal{F}_u)}{\eta_u} = \frac{X_u \eta_u}{\eta_u} = X_u$$

for any  $0 \leq u \leq t \leq T$ . We conclude that  $X$  is an  $\mathcal{F}$ -martingale under  $\mathbb{Q}$ . The proof of the converse implication goes along the same lines. ■